many key PCM lemmas

steel/Zeta.Steel.GhostSharedMap.fsti
@@ -21,7 +21,6 @@ let initial_map (#k:eqtype) (#v:Type) (#p:preorder v)
 [@@erasable]
 noeq
 type knowledge (k:eqtype) (v:Type) (p:preorder v) =
-  | Full     : kmap k v p -> knowledge k v p
   | Owns     : kmap k v p -> knowledge k v p
   | Nothing  : knowledge k v p
 
@@ -57,32 +56,12 @@ let kmap_composable (#k:eqtype) (#v:Type) (#p:preorder v) (m0 m1: kmap k v p)
    : prop
    = forall k. kmap_composable_k m0 m1 k
 
-let full_kmap_composable_k (#k:eqtype) (#v:Type) (#p:preorder v) (full:kmap k v p) (m1: kmap k v p) (key:k)
-  : prop
-  = let p0, v0 = Map.sel full key in
-    let p1, v1 = Map.sel m1 key in
-    perm_opt_composable p0 p1   /\
-    (match p1 with
-     | None -> v0 `extends` v1
-     | Some _ -> v0 == v1)
-
-let full_kmap_composable (#k:eqtype) (#v:Type) (#p:preorder v) (full:kmap k v p) (m1: kmap k v p)
-  : prop
-  = forall k. full_kmap_composable_k full m1 k
-
 let composable #k #v #p
   : symrel (knowledge k v p)
   = fun (k0 k1:knowledge k v p) ->
     match k0, k1 with
     | Nothing, _
     | _, Nothing -> True
-
-    | Full _, Full _ ->
-      False
-
-    | Full m, Owns m'
-    | Owns m', Full m ->
-      full_kmap_composable m m'
 
     | Owns m, Owns m' ->
       kmap_composable m m'
@@ -154,10 +133,6 @@ let compose #k #v #p (k0:knowledge k v p)
     | Nothing, k
     | k, Nothing -> k
 
-    | Full m, Owns m'
-    | Owns m', Full m ->
-      Full (compose_kmaps m m')
-
     | Owns m, Owns m' ->
       Owns (compose_kmaps m m')
 
@@ -182,70 +157,6 @@ let kmap_composable_assoc_r #k #v #p (k0 k1 k2: kmap k v p)
   = ()
 
 
-let full_kmap_composable_assoc_r_0 #k #v #p (k0 k1 k2: kmap k v p)
-  : Lemma
-    (requires
-           full_kmap_composable k0 k1 /\
-           full_kmap_composable (compose_kmaps k0 k1) k2)
-    (ensures
-           kmap_composable k1 k2 /\
-           full_kmap_composable k0 (compose_kmaps k1 k2))
-  = ()
-
-
-let full_kmap_composable_assoc_r_1 #k #v #p (k0 k1 k2: kmap k v p)
-  : Lemma
-    (requires
-           full_kmap_composable k1 k0 /\
-           full_kmap_composable (compose_kmaps k0 k1) k2)
-    (ensures
-           full_kmap_composable k1 k2 /\
-           full_kmap_composable (compose_kmaps k1 k2) k0)
-  = ()
-
-let full_kmap_composable_assoc_r_2 #k #v #p (k0 k1 k2: kmap k v p)
-  : Lemma
-    (requires
-           kmap_composable k1 k0 /\
-           full_kmap_composable k2 (compose_kmaps k0 k1))
-    (ensures
-           full_kmap_composable k2 k1 /\
-           full_kmap_composable (compose_kmaps k1 k2) k0)
-  = ()
-
-
-
-let full_kmap_composable_assoc_l_0 #k #v #p (k0 k1 k2: kmap k v p)
-  : Lemma
-    (requires
-           kmap_composable k1 k2 /\
-           full_kmap_composable k0 (compose_kmaps k1 k2))
-    (ensures
-           full_kmap_composable k0 k1 /\
-           full_kmap_composable (compose_kmaps k0 k1) k2)
-  = ()
-
-
-let full_kmap_composable_assoc_l_1 #k #v #p (k0 k1 k2: kmap k v p)
-  : Lemma
-    (requires
-           full_kmap_composable k1 k2 /\
-           full_kmap_composable (compose_kmaps k1 k2) k0)
-    (ensures
-           full_kmap_composable k1 k0 /\
-           full_kmap_composable (compose_kmaps k0 k1) k2)
-  = ()
-
-let full_kmap_composable_assoc_l_2 #k #v #p (k0 k1 k2: kmap k v p)
-  : Lemma
-    (requires
-           full_kmap_composable k2 k1 /\
-           full_kmap_composable (compose_kmaps k1 k2) k0)
-    (ensures
-           kmap_composable k1 k0 /\
-           full_kmap_composable k2 (compose_kmaps k0 k1))
-  = ()
-
 let composable_assoc_r #k #v #p (k0 k1 k2: knowledge k v p)
   : Lemma
     (requires  composable k0 k1 /\
@@ -257,29 +168,8 @@ let composable_assoc_r #k #v #p (k0 k1 k2: knowledge k v p)
     | Nothing, _, _
     | _, Nothing, _
     | _, _, Nothing -> ()
-    | _ ->
-      (match k0 with
-       | Full m0 -> (
-         match k1, k2 with
-         | Owns m1, Owns m2 ->
-           full_kmap_composable_assoc_r_0 m0 m1 m2
-         | Owns m1, Full m2 -> ()
-         | Full m1, Owns m2 -> ()
-         | Full m1, Full m2 -> ()
-       )
-
-       | Owns m0 -> (
-         match k1, k2 with
-         | Owns m1, Owns m2 ->
-           kmap_composable_assoc_r m0 m1 m2
-         | Owns m1, Full m2 ->
-           full_kmap_composable_assoc_r_2 m0 m1 m2
-         | Full m1, Owns m2 ->
-           full_kmap_composable_assoc_r_1 m0 m1 m2
-         | Full m1, Full m2 -> ()
-       )
-      )
-
+    | Owns m0, Owns m1, Owns m2 ->
+      kmap_composable_assoc_r m0 m1 m2
 
 let composable_assoc_l #k #v #p (k0 k1 k2: knowledge k v p)
   : Lemma
@@ -292,28 +182,8 @@ let composable_assoc_l #k #v #p (k0 k1 k2: knowledge k v p)
     | Nothing, _, _
     | _, Nothing, _
     | _, _, Nothing -> ()
-    | _ ->
-      (match k0 with
-       | Full m0 -> (
-         match k1, k2 with
-         | Owns m1, Owns m2 ->
-           full_kmap_composable_assoc_l_0 m0 m1 m2
-         | Owns m1, Full m2 -> ()
-         | Full m1, Owns m2 -> ()
-         | Full m1, Full m2 -> ()
-       )
-
-       | Owns m0 -> (
-         match k1, k2 with
-         | Owns m1, Owns m2 ->
-           kmap_composable_assoc_l m0 m1 m2
-         | Owns m1, Full m2 ->
-           full_kmap_composable_assoc_l_2 m0 m1 m2
-         | Full m1, Owns m2 ->
-           full_kmap_composable_assoc_l_1 m0 m1 m2
-         | Full m1, Full m2 -> ()
-       )
-      )
+    | Owns m0, Owns m1, Owns m2 ->
+      kmap_composable_assoc_l m0 m1 m2
 
 
 let p0 #k #v #p : pcm' (knowledge k v p) = {
@@ -321,43 +191,6 @@ let p0 #k #v #p : pcm' (knowledge k v p) = {
   op=compose;
   one=Nothing
 }
-
-let kmap_of_knowledge #k #v #p (kn:knowledge k v p { ~(Nothing? kn) })
-  : GTot (kmap k v p)
-  = match kn with
-    | Owns m
-    | Full m -> m
-
-
-let pcm #k #v #p : pcm (knowledge k v p) = {
-  p = p0;
-  comm = (fun _ _ -> ());
-  assoc = (fun k0 k1 k2 ->
-             composable_assoc_l k0 k1 k2;
-             match k0, k1, k2 with
-             | Nothing, _, _
-             | _, Nothing, _
-             | _, _, Nothing -> ()
-             | _ ->
-               compose_maps_assoc (kmap_of_knowledge k0)
-                                  (kmap_of_knowledge k1)
-                                  (kmap_of_knowledge k2));
-  assoc_r = (fun k0 k1 k2 ->
-               composable_assoc_r k0 k1 k2;
-               match k0, k1, k2 with
-               | Nothing, _, _
-               | _, Nothing, _
-               | _, _, Nothing -> ()
-               | _ ->
-                 compose_maps_assoc_r (kmap_of_knowledge k0)
-                                      (kmap_of_knowledge k1)
-                                      (kmap_of_knowledge k2));
-  is_unit = (fun _ -> ());
-  refine = (fun x -> Full? x == true);
-}
-
-let tmap (k:eqtype) (v:Type0) (c:preorder v) = Map.t k (hist c)
-
 
 let kmap_perm_of (#k:eqtype)
                  (#v:Type)
@@ -372,6 +205,40 @@ let kmap_owns_key (#k:eqtype)
                   (m:kmap k v p)
                   (key:k)
     = kmap_perm_of m key == Some full
+
+let full #k #v #p (kn:knowledge k v p)
+  : prop
+  = match kn with
+    | Nothing -> False
+    | Owns km -> forall k. kmap_owns_key km k
+
+let pcm #k #v #p : pcm (knowledge k v p) = {
+  p = p0;
+  comm = (fun k0 k1 ->
+             match k0, k1 with
+             | Nothing, _
+             | _, Nothing -> ()
+             | Owns m0, Owns m1 ->
+               compose_kmaps_comm m0 m1);
+  assoc = (fun k0 k1 k2 ->
+             composable_assoc_l k0 k1 k2;
+             match k0, k1, k2 with
+             | Nothing, _, _
+             | _, Nothing, _
+             | _, _, Nothing -> ()
+             | Owns m0, Owns m1, Owns m2 ->
+               compose_maps_assoc m0 m1 m2);
+  assoc_r = (fun k0 k1 k2 ->
+               composable_assoc_r k0 k1 k2;
+               match k0, k1, k2 with
+               | Nothing, _, _
+               | _, Nothing, _
+               | _, _, Nothing -> ()
+               | Owns m0, Owns m1, Owns m2 ->
+                 compose_maps_assoc_r m0 m1 m2);
+  is_unit = (fun _ -> ());
+  refine = full;
+}
 
 let kmap_value_of (#k:eqtype)
                   (#v:Type)
@@ -388,34 +255,117 @@ let kmap_update_key (#k:eqtype)
                     (value:vhist p)
     = Map.upd m key (kmap_perm_of m key, value)
 
+let update_key_hist (#k:eqtype)
+                    (#v:Type)
+                    (#p:preorder v)
+                    (m:kmap k v p)
+                    (key:k)
+                    (v1:vhist p {
+                      kmap_owns_key m key /\
+                      v1 `extends` kmap_value_of m key
+                    })
+  : frame_preserving_upd pcm (Owns m) (Owns (kmap_update_key m key v1))
+  = fun full_v ->
+      assert (full full_v);
+      assert (compatible pcm (Owns m) full_v);
+      let Owns full_m = full_v in
+      let m_res = kmap_update_key full_m key v1 in
+      let res = Owns m_res in
+      let m' = kmap_update_key m key v1 in
+      eliminate exists frame. composable (Owns m) frame /\ compose frame (Owns m) == full_v
+      returns (compatible pcm (Owns (kmap_update_key m key v1)) res)
+      with _. (
+           assert (composable (Owns (kmap_update_key m key v1)) frame);
+           match frame with
+           | Nothing -> ()
+           | Owns m_frame ->
+             assert (kmap_perm_of m_frame key == None);
+             assert (Map.equal (compose_kmaps m_frame m') m_res)
+      );
+      introduce forall (frame:_{composable (Owns m) frame}).
+                composable (Owns m') frame /\
+                (compose (Owns m) frame == full_v ==> compose (Owns m') frame == res)
+      with (
+        introduce _ /\ _
+        with ()
+        and introduce _ ==> _
+        with _. (
+          assert (compose (Owns m) frame == full_v);
+          match frame with
+          | Nothing -> ()
+          | Owns m_frame ->
+            assert (Map.equal (compose_kmaps m_frame m') m_res)
+        )
+      );
+      res
+
+let kmap_update_key_value (#k:eqtype)
+                          (#v:Type)
+                          (#p:preorder v)
+                          (m:kmap k v p)
+                          (key:k)
+                          (value:v { curval (kmap_value_of m key) `p` value })
+  : m':kmap k v p {
+                    curval (kmap_value_of m' key) == value /\
+                    kmap_value_of m' key `extends` kmap_value_of m key
+                  }
+  = let v = kmap_value_of m key in
+    kmap_update_key m key (extend_history v value)
+
 let update_key (#k:eqtype)
                (#v:Type)
                (#p:preorder v)
                (m:kmap k v p)
                (key:k)
-               (v1:vhist p {
+               (v1:v {
                  kmap_owns_key m key /\
-                 v1 `extends` kmap_value_of m key
+                 curval (kmap_value_of m key) `p` v1
                })
-  : frame_preserving_upd pcm (Owns m) (Owns (kmap_update_key m key v1))
-  = fun full_v ->
-      assert (Full? full_v);
-      assert (compatible pcm (Owns m) full_v);
-      let Full full_m = full_v in
-      let res = Full (kmap_update_key full_m key v1) in
-      let m' = (kmap_update_key m key v1) in
-      eliminate exists frame. composable (Owns m) frame /\ compose frame (Owns m) == full_v
-      returns (compatible pcm (Owns (kmap_update_key m key v1)) res)
-      with _. (
-           assume (composable (Owns (kmap_update_key m key v1)) frame);
-           assume (compose frame (Owns (kmap_update_key m key v1)) == res)
-      );
-      assert (compatible pcm (Owns (kmap_update_key m key v1)) res);
-      assume (forall (frame:_{composable (Owns m) frame}).
-                composable (Owns m') frame /\
-                (compose (Owns m) frame == full_v ==> compose (Owns m') frame == res));
-      res
+  : frame_preserving_upd pcm (Owns m) (Owns (kmap_update_key_value m key v1))
+  = update_key_hist m key (extend_history (kmap_value_of m key) v1)
 
+let ksnapshot (#k:eqtype) (#v:Type0) (#c:preorder v)
+             (m: kmap k v c)
+  : kmap k v c
+  = map_literal (fun k -> None, snd (Map.sel m k))
+
+let all_perms_ok (#k:eqtype)
+                 (#v:Type)
+                 (#p:preorder v)
+                 (m:kmap k v p)
+  = forall k. perm_opt_composable (kmap_perm_of m k) None
+
+
+let snapshot_lemma (#k:eqtype)
+                   (#v:Type)
+                   (#p:preorder v)
+                   (m:kmap k v p)
+  : Lemma (requires all_perms_ok m)
+          (ensures Owns m `composable` Owns (ksnapshot m))
+  = ()
+
+
+let snapshot_dup_lemma (#k:eqtype)
+                       (#v:Type)
+                       (#p:preorder v)
+                       (m:kmap k v p)
+  : Lemma (requires all_perms_ok m)
+          (ensures Owns (ksnapshot m) `composable` Owns (ksnapshot m))
+  = ()
+
+let update_snapshot_lemma (#k:eqtype)
+                          (#v:Type)
+                          (#p:preorder v)
+                          (m0 m1:kmap k v p)
+                          (key:k)
+  : Lemma (requires composable (Owns m0) (Owns m1) /\
+                    kmap_owns_key m0 key)
+          (ensures composable (Owns m0) (Owns (kmap_update_key m1 key (kmap_value_of m0 key))))
+  = ()
+
+////////////////////////////////////////////////////////////////////////////////
+
+let tmap (k:eqtype) (v:Type0) (c:preorder v) = Map.t k (hist c)
 
 val t (k:eqtype) (v:Type0) (c:preorder v) : Type0
 
@@ -440,11 +390,6 @@ val gather (#o:_)
   : STGhostT (_:unit { kmap_composable m0 m1 }) o
     (k_of t (Owns m0) `star` k_of t (Owns m1))
     (fun _ -> k_of t (Owns (compose_kmaps m0 m1)))
-
-let ksnapshot (#k:eqtype) (#v:Type0) (#c:preorder v)
-             (m: kmap k v c)
-  : kmap k v c
-  = map_literal (fun k -> None, snd (Map.sel m k))
 
 let snapshot (#k:eqtype) (#v:Type0) (#c:preorder v)
              (m: kmap k v c)
